regex.v
@@ -1,0 +1,263 @@
+Require Import List.
+Import ListNotations.
+Require Import Nat.
+Require Import Coq.Program.Wf.
+Require Import Coq.omega.Omega.
+
+Ltac inv H := inversion H; subst; clear H.
+
+(* Borrowed these from another paper, actually about regex derivatives *)
+Variable Sigma : Type.
+Variable x : Sigma.
+Variable y : Sigma.
+Variable z : Sigma.
+Variable Sigma_dec : forall (c c': Sigma), {c = c'} + {c <> c'}.
+Axiom Sigma_dec_refl : forall(T : Type) (p1 p2 : T) (a : Sigma), p1 = if Sigma_dec a a then p1 else p2.
+Definition String : Type := list Sigma.
+
+(* Didn't bother with Intersection and Complement yet *)
+Inductive regex : Type :=
+  | EmptySet
+  | EmptyStr
+  | Char (t : Sigma)
+  | App (r1 r2 : regex)
+  | Union (r1 r2 : regex)
+  | Star (r : regex).
+
+Inductive exp_match : String -> regex -> Prop :=
+  | MEmpty : exp_match [] EmptyStr
+  | MChar x : exp_match [x] (Char x)
+  | MApp s1 re1 s2 re2
+             (H1 : exp_match s1 re1)
+             (H2 : exp_match s2 re2) :
+             exp_match (s1 ++ s2) (App re1 re2)
+  | MUnionL s1 re1 re2
+                (H1 : exp_match s1 re1) :
+                exp_match s1 (Union re1 re2)
+  | MUnionR re1 s2 re2
+                (H2 : exp_match s2 re2) :
+                exp_match s2 (Union re1 re2)
+  | MStar0 re : exp_match [] (Star re)
+  (* | MStarChar a re
+                 (H1 : exp_match [a] re) :
+      exp_match [a] (Star re) *)
+  | MStarApp s1 s2 re
+                 (H1 : exp_match s1 re)
+                 (H2 : exp_match s2 (Star re)) :
+      exp_match (s1 ++ s2) (Star re).
+
+Fixpoint nullable (r : regex) : bool:=
+  match r with
+  | EmptySet => false
+  | EmptyStr => true
+  | Char _ => false
+  | App r1 r2 => andb (nullable r1) (nullable r2)
+  | Union r1 r2 => orb (nullable r1) (nullable r2)
+  | Star _ => true
+  end.
+
+Fixpoint nullify (r : regex) := if (nullable r) then EmptyStr else EmptySet.
+
+Fixpoint derivative (a : Sigma) (r : regex) :=
+  match r with
+  | EmptySet => EmptySet
+  | EmptyStr => EmptySet
+  | Char x => if Sigma_dec x a then EmptyStr else EmptySet
+  | App r1 r2 =>  Union (App (derivative a r1) r2) (App (nullify r1) (derivative a r2))
+  | Union r1 r2 => Union (derivative a r1) (derivative a r2)
+  | Star r => App (derivative a r) (Star r)
+  end.
+
+Fixpoint exp_matchb (s : String) (r : regex) :=
+  match s, r with
+  | [], _ => nullable r
+  | x::xs, _ => exp_matchb xs (derivative x r)
+  end.
+
+Lemma nil_right : forall(s : String), s ++ [] = s.
+Proof.
+  induction s.
+  - simpl. reflexivity.
+  - simpl. rewrite IHs. reflexivity.
+Qed.
+
+Lemma nil_left : forall(s : String), [] ++ s = s.
+Proof.
+  intros s. simpl. reflexivity.
+Qed.
+
+Lemma empty_app : forall(s1 s2 : String), s1 ++ s2 = [] -> s1 = [] /\ s2 = [].
+Proof.
+  intros s1 s2 H. destruct s1; destruct s2; try(simpl in H; discriminate).
+  - split; reflexivity.
+Qed.
+
+Lemma singleton_app : forall(a : Sigma) (s1 s2 : String),
+    s1 ++ s2 = [a] -> (s1 = [a] /\ s2 = []) \/ (s1 = [] /\ s2 = [a]).
+Proof.
+Admitted.
+
+Lemma mute_nullify : forall(r : regex),
+    nullable (nullify r) = nullable r.
+Proof.
+Admitted.
+
+Lemma Star_empty_empty : forall(s : String),
+    exp_match s (Star EmptyStr) -> s = [].
+Proof.
+Admitted.
+
+Theorem nullable_bridge : forall(r : regex),
+    true = nullable r <-> exp_match [] r.
+Proof.
+  intros r. split; intros H.
+  - induction r; try(simpl in H; discriminate).
+    + apply MEmpty.
+    + simpl in H. destruct (nullable r1); destruct (nullable r2); try(simpl in H; discriminate).
+      rewrite <- nil_left with (s := []). apply MApp.
+      * apply IHr1. reflexivity.
+      * apply IHr2. reflexivity.
+    + simpl in H.  destruct (nullable r1); destruct (nullable r2).
+      * apply MUnionL. apply IHr1. reflexivity.
+      * apply MUnionL. apply IHr1. reflexivity.
+      * apply MUnionR. apply IHr2. reflexivity.
+      * simpl in H. discriminate.
+    + apply MStar0.
+  - induction r.
+    + inversion H.
+    + simpl. reflexivity.
+    + inversion H.
+    + simpl. inversion H. apply empty_app in H1. destruct H1.
+      rewrite H1 in H3. rewrite H5 in H4.
+      apply IHr1 in H3. apply IHr2 in H4.
+      rewrite <- H3. rewrite <- H4. simpl. reflexivity.
+    + simpl. inversion H.
+      * apply IHr1 in H2. rewrite <- H2. destruct (nullable r2); simpl; reflexivity.
+      * apply IHr2 in H1. rewrite <- H1. destruct (nullable r1); simpl; reflexivity.
+    + simpl. reflexivity.
+Qed.
+
+Lemma foo0 : forall(s : String) (r : regex),
+    exp_match s r -> exp_match s (Star r).
+Proof.
+  intros s. induction s; intros r H.
+  - apply MStar0.
+  - rewrite <- nil_right with (s := a::s). apply MStarApp.
+    + apply H.
+    + apply MStar0.
+Qed.
+  
+Lemma foo1 : forall(a : Sigma) (r1 r2 : regex),
+    exp_match [a] (Star (App r1 r2)) ->
+    (exp_match [a] r1) \/
+    (exp_match [a] r2).
+Proof.
+Admitted.
+
+Lemma foo2 : forall(a : Sigma) (r1 r2 : regex),
+    exp_match [a] (Star (App r1 r2)) ->
+    (exp_match [a] r1 -> exp_match [] r2) /\
+    (exp_match [a] r2 -> exp_match [] r1).
+Proof.
+  intros a r1 r2 H. split; intros H1.
+  - inv H.
+    apply singleton_app in H0. destruct H0; destruct H.
+    + rewrite H in H3. inv H3. inv H4
+    + rewrite H in H3. Admitted.
+
+Theorem singleton_star_app : forall(a : Sigma) (r1 r2 : regex),
+    exp_match [a] (Star (App r1 r2)) ->
+    (exp_match [a] (Star r1) /\ exp_match [] r2) \/
+    (exp_match [a] (Star r2) /\ exp_match [] r1).
+Proof.
+  intros a r1 r2 H.
+  assert(H1 := H).
+  apply foo1 in H. apply foo2 in H1.
+  destruct H1. destruct H; assert(H2 := H); apply foo0 in H2.
+  - left. split.
+    + apply H2.
+    + apply H0. apply H.
+  - right. split.
+    + apply H2.
+    + apply H1. apply H.
+Qed.
+
+Lemma singleton_star : forall(a : Sigma) (r : regex),
+    exp_match [a] (Star r) -> exp_match [a] r.
+Proof.
+  intros a r H. induction r.
+  - inv H. inv H2.
+  - inv H. apply singleton_app in H1. destruct H1; destruct H.
+    + rewrite H in H2. inv H2.
+    + apply Star_empty_empty in H3. rewrite H0 in H3. discriminate.
+  - inv H. apply singleton_app in H1. destruct H1; destruct H.
+    + rewrite H in H2. rewrite H. rewrite H0. simpl. apply H2.
+    + rewrite H0 in H3. inv H3. inv H2.
+  - apply singleton_star_app in H. destruct H; destruct H.
+    + rewrite <- nil_right with (s := [a]). apply MApp.
+      * apply IHr1. apply H.
+      * apply H0.
+    + rewrite <- nil_left with (s := [a]). apply MApp.
+      * apply H0.
+      * apply IHr2. apply H.
+  - Admitted.
+                     
+Theorem der_matchb : forall(a : Sigma) (s : String) (r : regex),
+    true = exp_matchb (a::s) r <-> true = exp_matchb s (derivative a r).
+Proof.
+  intros a s r.
+  split; generalize dependent r; induction s; intros r H; simpl; simpl in H; apply H.
+Qed.
+
+Theorem der_match : forall(a : Sigma) (s : String) (r : regex),
+    exp_match (a::s) r <-> exp_match s (derivative a r).
+Proof.
+  intros a s r.
+  split.
+  {
+    generalize dependent r. induction s; intros r H.
+    - apply nullable_bridge. induction r.
+      + inv H.
+      + inv H.
+      + simpl. destruct (Sigma_dec t a).
+        * simpl. reflexivity.
+        * inv H. contradiction.
+      + inv H. apply singleton_app in H1.
+        destruct H1; destruct H; rewrite H in H3; rewrite H0 in H4.
+        * apply nullable_bridge in H4. apply IHr1 in H3.
+          simpl. rewrite <- H3. rewrite <- H4.
+          destruct (andb (nullable (nullify r1)) (nullable (derivative a r2))); simpl; reflexivity.
+        * apply nullable_bridge in H3. apply IHr2 in H4.
+          simpl. rewrite mute_nullify. rewrite <- H3. rewrite <- H4.
+          destruct (andb (nullable (derivative a r1)) (nullable r2)); simpl; reflexivity.
+      + inv H.
+        * simpl. apply IHr1 in H2. rewrite <- H2.
+          destruct (nullable (derivative a r2)); simpl; reflexivity.
+        * simpl. apply IHr2 in H1. rewrite <- H1.
+          destruct (nullable (derivative a r1)); simpl; reflexivity.
+      + 
+
+        simpl. apply singleton_star in H. apply IHr in H. rewrite <- H. reflexivity.
+    - 
+  }
+  {
+    admit.
+  }
+Admitted.
+
+Theorem match_iff_matchb : forall(s : String) (r : regex),
+    true = exp_matchb s r <-> exp_match s r.
+Proof.
+  intros s r. split.
+  {
+    generalize dependent r. induction s; intros r H.
+    - simpl in H. apply nullable_bridge. apply H.
+    - apply der_match. apply der_matchb in H. apply IHs. apply H.
+  }
+  {
+    generalize dependent r. induction s; intros r H.
+    - simpl. apply nullable_bridge. apply H.
+    - apply der_match in H. apply der_matchb. apply IHs in H. apply H.
+  }
+Qed.
+
